Phi_System/IDE_CP_Reasoning1.thy
@@ -1,0 +1,249 @@
+chapter \<open>Reasoning Processes in IDE-CP - Part I\<close>
+
+text \<open>The part includes small process that can be built without infrastructure of
+  IDE-CP, and declarations of other large process.\<close>
+
+theory IDE_CP_Reasoning1
+  imports Spec_Framework
+begin
+
+section \<open>Normalization of Assertions\<close>
+
+consts assertion_simplification :: mode
+
+named_theorems assertion_simps \<open>Simplification rules normalizing an assertion.
+  It is applied before ToSA process.\<close>
+
+\<phi>reasoner assertion_simplification 1200
+  (\<open>Simplify assertion_simplification ?X' ?X\<close>)
+  = ((simp only: assertion_simps)?, rule Simplify_I)
+
+lemmas [assertion_simps] =
+  mult_zero_right mult_zero_left mult_1_right mult_1_left add_0_right add_0_left zero_fun
+  zero_fun_def[symmetric] plus_fun Subjection_Zero ExSet_const FOCUS_TAG_def ExSet_0
+
+
+section \<open>Annotations Guiding the Reasoning\<close>
+
+subsection \<open>Small Annotations\<close>
+
+subsubsection \<open>Matches\<close>
+
+definition Assertion_Matches :: \<open>'a set \<Rightarrow> 'a set \<Rightarrow> 'a set\<close> (infixl "<matches>" 18)
+  where \<open>(S <matches> pattern) = S\<close>
+
+text \<open>The annotation marking on a target \<^term>\<open>Y <matches> A\<close> in a ToA or a view shift
+  restricts that the source have to first match pattern \<open>A\<close>.\<close>
+
+lemma [\<phi>reason 2000]:
+  \<open>Matches X A \<Longrightarrow> X \<^bold>i\<^bold>m\<^bold>p\<^bold>l\<^bold>i\<^bold>e\<^bold>s Y \<^bold>a\<^bold>n\<^bold>d P \<Longrightarrow> X \<^bold>i\<^bold>m\<^bold>p\<^bold>l\<^bold>i\<^bold>e\<^bold>s (Y <matches> A) \<^bold>a\<^bold>n\<^bold>d P\<close>
+  unfolding Assertion_Matches_def .
+
+lemma [\<phi>reason 2000]:
+  \<open>Matches X A \<Longrightarrow> \<^bold>v\<^bold>i\<^bold>e\<^bold>w X \<longmapsto> Y \<^bold>w\<^bold>i\<^bold>t\<^bold>h P \<Longrightarrow> \<^bold>v\<^bold>i\<^bold>e\<^bold>w X \<longmapsto> (Y <matches> A) \<^bold>w\<^bold>i\<^bold>t\<^bold>h P\<close>
+  unfolding Assertion_Matches_def .
+
+
+section \<open>Small Reasoning Process\<close>
+
+subsubsection \<open>Semantic Expansion of \<phi>-Types\<close>
+
+consts MODE_\<phi>EXPN :: mode \<comment> \<open>relating to named_theorems \<open>\<phi>expn\<close>\<close>
+
+abbreviation \<phi>expn_Premise ("<\<phi>expn> _" [26] 26) where \<open>\<phi>expn_Premise \<equiv> Premise MODE_\<phi>EXPN\<close>
+
+\<phi>reasoner \<phi>expn_Premise 10 (\<open><\<phi>expn> ?P\<close>)
+  = (rule Premise_I; simp add: \<phi>expns)
+
+text \<open>Antecedent \<^prop>\<open><\<phi>expn> P\<close> indicates the reasoner solving the premise \<^prop>\<open>P\<close> using
+  simplification rules of \<open>\<phi>expns\<close>.\<close>
+
+subsubsection \<open>Name tag by type\<close>
+
+(*TODO: elaborate this*)
+
+datatype ('x, 'name) named (infix "<named>" 30) = tag 'x
+
+syntax "__named__" :: \<open>logic \<Rightarrow> tuple_args \<Rightarrow> logic\<close> (infix "<<named>>" 25)
+
+
+ML_file \<open>library/name_by_type.ML\<close>
+
+text \<open>It is a tool to annotate names on a term, e.g. \<^term>\<open>x <<named>> a, b\<close>.
+  The name tag is useful in lambda abstraction (including quantification) because the
+  name of an abstraction variable is not preserved in many transformation especially
+  simplifications. The name can be useful in the deductive programming, e.g. universally
+  quantified variables in a sub-procedure like
+  \[ \<open>\<forall>x y. proc f \<lbrace> VAL x \<Ztypecolon> T\<heavy_comma> VAL y \<Ztypecolon> U \<longmapsto> any \<rbrace> \<Longrightarrow> any'\<close> \]
+  When starting to write the sub-procedure f by command \<open>\<medium_left_bracket>\<close>, \<phi>-system fixes variables x and y
+    with the name of x and y. The name of x and y then are significant for programming.
+  To preserve the name, we use \<^typ>\<open>'any <named> '\<phi>name_x \<times> '\<phi>name_y\<close>,
+    \<^prop>\<open>\<forall>(x :: 'any <named> '\<phi>name_x). sth\<close>.
+  We use free type variable to annotate it because it is most stable. No transformation
+    changes the name of a free type variable.
+
+  This feature is mostly used in \<^emph>\<open>Expansion of Quantification\<close> given in the immediate subsection.
+  Therefore we put this part in the subsection of reasoning jobs, though itself is not related to
+  any reasoning work.
+\<close>
+
+lemma named_forall: "All P \<longleftrightarrow> (\<forall>x. P (tag x))" by (metis named.exhaust)
+lemma named_exists: "Ex P \<longleftrightarrow> (\<exists>x. P (tag x))" by (metis named.exhaust)
+lemma [simp]: "tag (case x of tag x \<Rightarrow> x) = x" by (cases x) simp
+lemma named_All: "(\<And>x. PROP P x) \<equiv> (\<And>x. PROP P (tag x))"
+proof fix x assume "(\<And>x. PROP P x)" then show "PROP P (tag x)" .
+next fix x :: "'a <named> 'b" assume "(\<And>x. PROP P (tag x))" from \<open>PROP P (tag (case x of tag x \<Rightarrow> x))\<close> show "PROP P x" by simp
+qed
+
+lemma named_ExSet: "(ExSet T) = (\<exists>*c. T (tag c) )" by (auto simp add: named_exists \<phi>expns)
+
+
+subsubsection \<open>Expansion of Quantification\<close>
+
+definition \<open>eoq__fst = fst\<close>
+definition \<open>eoq__snd = snd\<close>
+
+named_theorems named_expansion \<open>Rewriting rules expanding named quantification.\<close>
+
+lemma eoq__fst[unfolded atomize_eq[symmetric], named_expansion]:
+        \<open>eoq__fst (x,y) = x\<close> unfolding eoq__fst_def by simp
+lemma eoq__snd[unfolded atomize_eq[symmetric], named_expansion]:
+        \<open>eoq__snd (x,y) = y\<close> unfolding eoq__snd_def by simp
+
+lemmas [unfolded atomize_eq[symmetric], named_expansion] =
+  Product_Type.prod.case named.case id_apply
+
+ML_file "./library/QuantExpansion.ML"
+
+simproc_setup named_forall_expansion ("All (P :: 'a <named> 'names \<Rightarrow> bool)") =
+  \<open>K (QuantExpansion.simproc_of QuantExpansion.forall_expansion)\<close>
+
+simproc_setup named_exSet_expansion ("ExSet (P :: 'a <named> 'names \<Rightarrow> 'b set)") =
+  \<open>K (fn ctx => fn cterms => QuantExpansion.simproc_of QuantExpansion.ExNu_expansion ctx cterms)\<close>
+
+simproc_setup named_pureAll_expansion ("Pure.all (P :: 'a <named> 'names \<Rightarrow> prop)") =
+  \<open>K (QuantExpansion.simproc_of QuantExpansion.pure_All_expansion)\<close>
+
+
+subsubsection \<open>Rename \<lambda>-Abstraction\<close>
+
+definition rename_abstraction :: \<open>'\<phi>name_name itself \<Rightarrow> 'a \<Rightarrow> 'a \<Rightarrow> bool\<close>
+  where \<open>rename_abstraction name origin_abs named_abs \<longleftrightarrow> (origin_abs = named_abs)\<close>
+
+lemma rename_abstraction:
+  \<open>rename_abstraction name X X\<close>
+  unfolding rename_abstraction_def ..
+
+\<phi>reasoner_ML rename_abstraction 1100 (\<open>rename_abstraction TYPE(?'name) ?Y ?Y'\<close>) =
+\<open>fn (ctxt, sequent) =>
+  case Thm.major_prem_of sequent
+    of \<^const>\<open>Trueprop\<close> $ (Const (\<^const_name>\<open>rename_abstraction\<close>, _)
+                $ (Const (\<^const_name>\<open>Pure.type\<close>, Type(\<^type_name>\<open>itself\<close>, [name'])))
+                $ Abs(_,ty,body)
+                $ Var Y'') =>
+      let
+        val name = case Phi_Syntax.dest_name_tylabels name'
+                     of [x] => x
+                      | _ => raise TYPE ("only one name is expected", [name'], [])
+        val Y' = Abs(name, ty, body) |> Thm.cterm_of ctxt
+        val sequent = @{thm rename_abstraction} RS Thm.instantiate (TVars.empty, Vars.make [(Y'',Y')]) sequent
+      in
+        Seq.single (ctxt, sequent)
+      end
+     | term => raise THM ("Bad shape of rename_abstraction antecedent", 0, [sequent])
+\<close>
+
+
+subsubsection \<open>\<lambda>-Abstraction Tag\<close>
+
+definition "lambda_abstraction" :: " 'a \<Rightarrow> 'b \<Rightarrow> ('a \<Rightarrow> 'b) \<Rightarrow> bool "
+  where "lambda_abstraction x Y Y' \<longleftrightarrow> Y' x = Y"
+
+lemma lambda_abstraction: "lambda_abstraction x (Y' x) Y'"
+  unfolding lambda_abstraction_def ..
+
+lemma [\<phi>reason 1200 for \<open>lambda_abstraction (?x,?y) ?fx ?f\<close>]:
+  \<open> lambda_abstraction y fx f1
+\<Longrightarrow> lambda_abstraction x f1 f2
+\<Longrightarrow> lambda_abstraction (x,y) fx (case_prod f2)\<close>
+  unfolding lambda_abstraction_def by simp
+
+ML \<open>Name.variant "" Name.context\<close>
+
+\<phi>reasoner_ML lambda_abstraction 1100 ("lambda_abstraction ?x ?Y ?Y'") = \<open>fn (ctxt, sequent) =>
+  let
+    val (Vs, _, \<^const>\<open>Trueprop\<close> $ (Const (\<^const_name>\<open>lambda_abstraction\<close>, _) $ x $ Y $ _))
+      = Phi_Help.leading_antecedent (Thm.prop_of sequent)
+    val Y' = Abs("", fastype_of x, abstract_over (x, Y))
+    val idx = Thm.maxidx_of sequent
+    val vars = map Var (List.tabulate (length Vs, (fn i => ("v", i+idx))) ~~ map snd Vs)
+    fun subst X = Term.subst_bounds (vars, X)
+    val rule = Drule.infer_instantiate ctxt
+                  (map (apsnd (Thm.cterm_of ctxt)) [(("x",0), subst x), (("Y'",0),subst Y')])
+                  @{thm lambda_abstraction}
+  in
+    Seq.single (ctxt, rule RS sequent)
+  end
+\<close>
+
+lemma [\<phi>reason 1200 for \<open>lambda_abstraction (tag ?x) ?fx ?f\<close>]:
+  \<open> lambda_abstraction x fx f
+\<Longrightarrow> rename_abstraction TYPE('name) f f'
+\<Longrightarrow> lambda_abstraction (tag x :: 'any <named> 'name) fx (case_named f')\<close>
+  unfolding lambda_abstraction_def rename_abstraction_def by simp
+
+
+
+section \<open>Declaration of Large Processes\<close>
+
+subsection \<open>Transformation of State Abstraction (ToSA)\<close>
+
+text \<open>
+  Supporting either view shift \<open>\<^bold>v\<^bold>i\<^bold>e\<^bold>w X \<longmapsto> Y \<^bold><\<^bold>a\<^bold>c\<^bold>t\<^bold>i\<^bold>o\<^bold>n\<^bold>> ToSA\<close> or
+  implication \<open>X \<^bold>i\<^bold>m\<^bold>p\<^bold>l\<^bold>i\<^bold>e\<^bold>s Y \<^bold><\<^bold>a\<^bold>c\<^bold>t\<^bold>i\<^bold>o\<^bold>n\<^bold>> ToSA\<close>,
+  ToSA is a reasoning process of Transformation of Abstraction (ToA) for
+  assertions of (fictional) computation state.
+\<close>
+
+consts ToSA' :: \<open>bool \<comment> \<open>whether to reason deeper transformation for each desired \<phi>-type
+                          by invoking more time-consuming reasoning process,
+                          or just apply unification to match the desired.\<close>
+              \<Rightarrow> mode\<close>
+
+text \<open>The boolean flag indicates whether to reason the transformation of \<phi>-types in depth.
+For \<open>X\<^sub>1 * \<cdots> * X\<^sub>n \<^bold>i\<^bold>m\<^bold>p\<^bold>l\<^bold>i\<^bold>e\<^bold>s Y\<^sub>1 * \<cdots> * Y\<^sub>m \<^bold><\<^bold>a\<^bold>c\<^bold>t\<^bold>i\<^bold>o\<^bold>n\<^bold>> ToSA' ?flag\<close>,
+
+\<^item> If the flag is turned on, for every desired \<phi>-Type \<^term>\<open>Y\<^sub>i\<close>, the reasoner
+  infers in depth whether some source \<phi>-Type \<^term>\<open>X\<^sub>j\<close> can be transformed into \<^term>\<open>Y\<^sub>i\<close>,
+  by invoking any configured reasoning rules bound on the type of \<^term>\<open>Y\<^sub>i\<close>.
+
+\<^item> If the flag is turned off, such in-depth inference is not applied, so the
+  reasoning succeeds only if for every desired \<phi>-Type \<^term>\<open>Y\<^sub>i\<close> there is another
+  \<^term>\<open>X\<^sub>j\<close> that unifies \<^term>\<open>Y\<^sub>i\<close>.
+
+The the flag is turned off, obviously the performance can be improved a lot though
+the reasoning is weaker.
+\<close>
+
+abbreviation \<open>ToSA \<equiv> ToSA' True\<close>
+
+lemma [\<phi>reason 3000 for \<open>\<^bold>v\<^bold>i\<^bold>e\<^bold>w ?X \<longmapsto> ?X' \<^bold>w\<^bold>i\<^bold>t\<^bold>h ?P \<^bold><\<^bold>a\<^bold>c\<^bold>t\<^bold>i\<^bold>o\<^bold>n\<^bold>> ToSA' ?mode\<close>]:
+  \<open>\<^bold>v\<^bold>i\<^bold>e\<^bold>w X \<longmapsto> X \<^bold><\<^bold>a\<^bold>c\<^bold>t\<^bold>i\<^bold>o\<^bold>n\<^bold>> ToSA' mode\<close>
+  unfolding Action_Tag_def using \<phi>view_refl .
+
+subsection \<open>Removing Values\<close>
+
+definition \<open>Remove_Values (Input::assn) (Output::assn) \<longleftrightarrow> (Input \<^bold>i\<^bold>m\<^bold>p\<^bold>l\<^bold>i\<^bold>e\<^bold>s Output)\<close>
+
+text \<open>The process \<^prop>\<open>Remove_Values Input Output\<close> removes value assertions \<open>x \<Ztypecolon> \<^bold>v\<^bold>a\<^bold>l T\<close>
+  from the assertion \<open>Input\<close>. Bounded values such the return value of a procedure are not removed.\<close>
+
+subsection \<open>Collects all Values in an Assertion / from the State Sequent\<close>
+
+lemma Val_inhabited_collect:
+  \<open> Inhabited (x \<Ztypecolon> \<^bold>v\<^bold>a\<^bold>l[v] T) \<Longrightarrow> (sem_value.dest v \<in> (x \<Ztypecolon> T) \<Longrightarrow> C) \<Longrightarrow> C \<close>
+  unfolding Inhabited_def by (clarsimp simp add: \<phi>expns)
+
+
+
+end
